Adapting to new universe instances

template-rocq/src/constr_quoter.ml
@@ -205,9 +205,11 @@ struct
          | Some x -> constr_mkApp (tLevelVar, [| quote_int x |])
          | None -> constr_mkApp (tLevel, [| string_of_level l |])
 
+  let of_level l = constr_mkApp (tof_level, [| l |])
+
   let quote_universe s =
     match Univ.Universe.level s with
-      Some l -> constr_mkApp (tof_level, [| quote_level l |])
+      Some l -> of_level (quote_level l)
     | _ -> let levels = List.map (fun (l,i) -> pairl tlevel tnat (quote_level l) (quote_int i)) (Universe.repr s) in
            let hd = List.hd levels in
            let tl = to_coq_list (prodl tlevel tnat) (List.tl levels) in
@@ -220,15 +222,16 @@ struct
 
   let quote_constraint_type (c : Univ.constraint_type) =
     match c with
-    | Lt -> Lazy.force tunivLt
-    | Le -> Lazy.force tunivLe0
+    | Lt -> Lazy.force tunivLe (* BEWARE: this is fixed in quote_univ_constraint *)
+    | Le -> Lazy.force tunivLe
     | Eq -> Lazy.force tunivEq
 
   let quote_univ_constraint ((l1, ct, l2) : Univ.univ_constraint) =
     let l1 = quote_level l1 in
     let l2 = quote_level l2 in
+    let u1 = if ct == Lt then constr_mkApp (tsucc, [| of_level l1 |]) else of_level l1 in
     let ct = quote_constraint_type ct in
-    constr_mkApp (tmake_univ_constraint, [| l1; ct; l2 |])
+    constr_mkApp (tmake_univ_constraint, [| u1; ct; of_level l2 |])
 
   let quote_univ_level u = quote_level u
   (* todo : can be deduced from quote_level, hence shoud be in the Reify module *)
@@ -333,7 +336,7 @@ struct
     let inst' = quote_univ_instance UVars.Instance.empty in
     let const' = quote_univ_constraints (fst (UGraph.constraints_of_universes g)) in
     let uctx = constr_mkApp (tUContextmake, [|inst' ; const'|]) in
-    constr_mkApp (tadd_global_constraints, [|constr_mkApp (cMonomorphic_ctx, [| uctx |]); Lazy.force tinit_graph|])
+    constr_mkApp (tadd_global_constraints, [|Lazy.force tinit_graph; constr_mkApp (cMonomorphic_ctx, [| uctx |])|])
 
 
   let sprop =
