pcuic/theories/PCUICCumulativitySpec.v
@@ -28,7 +28,7 @@ Definition cumul_predicate_dep {cumul cumul_universe Γ p p'}
 
 Lemma cumul_predicate_undep {cumul cumul_universe Γ p p' H cumul' cumul_universe'} :
   @cumul_predicate cumul' cumul_universe' Γ p p' <~>
-  @cumul_predicate_dep cumul cumul_universe Γ p p' H (fun Γ p p' _ => cumul' Γ p p') (fun x y _ => on_rel cumul_universe' Universe.make' x y).
+  @cumul_predicate_dep cumul cumul_universe Γ p p' H (fun Γ p p' _ => cumul' Γ p p') (fun x y _ => on_rel cumul_universe' Universe.of_level x y).
 Proof.
   cbv [cumul_predicate cumul_predicate_dep cmp_universe_instance cmp_universe_instance_dep] in *.
   split; intro; repeat destruct ?; subst; rdest; try assumption.
@@ -380,7 +380,7 @@ Lemma cumulSpec0_rect :
     (forall (Γ : context) (pb : conv_pb) (indn : case_info) (p p' : predicate term)
             (c c' : term) (brs brs' : list (branch term))
             (Hp : cumul_predicate (fun Γ => cumulSpec0 Σ Γ Conv) (compare_universe Σ Conv) Γ p p')
-            (_ : cumul_predicate_dep Hp (fun Γ => P cf Σ Γ Conv) (fun l l' _ => on_rel (fun _ _ => True) Universe.make' l l'))
+            (_ : cumul_predicate_dep Hp (fun Γ => P cf Σ Γ Conv) (fun l l' _ => on_rel (fun _ _ => True) Universe.of_level l l'))
             (Hc : cumulSpec0 Σ Γ Conv c c') (_ : P cf Σ Γ Conv c c' Hc)
             (Hbody : cumul_branches (fun Γ => cumulSpec0 Σ Γ Conv) Γ p brs brs')
             (_ : All2_dep
@@ -654,7 +654,7 @@ Lemma convSpec0_ind_all :
       (forall (Γ : context) (indn : case_info) (p p' : predicate term)
               (c c' : term) (brs brs' : list (branch term))
               (Hp : cumul_predicate (fun Γ => cumulSpec0 Σ Γ Conv) (compare_universe Σ Conv) Γ p p')
-              (_ : cumul_predicate_dep Hp (fun Γ => P cf Σ Γ Conv) (fun l l' _ => on_rel (fun _ _ => True) Universe.make' l l'))
+              (_ : cumul_predicate_dep Hp (fun Γ => P cf Σ Γ Conv) (fun l l' _ => on_rel (fun _ _ => True) Universe.of_level l l'))
               (Hc : cumulSpec0 Σ Γ Conv c c') (_ : P cf Σ Γ Conv c c' Hc)
               (Hbody : cumul_branches (fun Γ => cumulSpec0 Σ Γ Conv) Γ p brs brs')
               (_ : All2_dep
