pcuic/theories/PCUICValidity.v
@@ -335,7 +335,7 @@ Section Validity.
       depelim X0; depelim X1; simp prim_type; cbn in *.
       1-3:destruct H1 as [hty hbod huniv]; eapply has_sort_isType with (s := _@[[]]); change (tSort ?s@[[]]) with (tSort s)@[[]];
           rewrite <- hty; refine (type_Const _ _ _ [] _ wfΓ H0 _); rewrite huniv //.
-      set (s := sType (Universe.make' (array_level a))).
+      set (s := sType (Universe.of_level (array_level a))).
       destruct H1 as [hty' hbod huniv].
       eapply has_sort_isType with s.
       eapply (type_App _ _ _ _ (tSort s) (tSort s)); tea; cycle 1.
