template-rocq/theories/TemplateMonad/Core.v
@@ -231,9 +231,9 @@ Definition tmFix@{a b t u} {A : Type@{a}} {B : Type@{b}} (f : (A -> TemplateMona
   := f (fun a
         => (qA <- tmQuote A;;
             qB <- tmQuote B;;
-            qa <- tmQuoteLevel@{a _ _};;
-            qb <- tmQuoteLevel@{b _ _};;
-            qt <- tmQuoteLevel@{t _ _};;
-            qu <- tmQuoteLevel@{u _ _};;
+            qa <- tmQuoteUniverse@{a _ _};;
+            qb <- tmQuoteUniverse@{b _ _};;
+            qt <- tmQuoteUniverse@{t _ _};;
+            qu <- tmQuoteUniverse@{u _ _};;
             let self := tConst (MPfile ["Core"; "TemplateMonad"; "Template"; "MetaRocq"], "tmFix'")%bs [qa;qb;qt;qu] in
             @tmFix'@{a b t u} A B (mkApps self [qA; qB]) f a)).
